further renaming of Obs

src/ml/interpreter.ml
@@ -22,7 +22,7 @@ let rec step m =
   | SS.E.Fin v -> print_int_dvalue v
   | SS.E.Err s -> failwith (Printf.sprintf "ERROR: %s" (Camlcoq.camlstring_of_coqstring s))
   | SS.E.Ret _ -> failwith "should be impossible"
-  | SS.E.Eff (SS.E.Call(args, k)) -> ()
+  | SS.E.Eff (SS.E.Call(f, args, k)) -> ()
   | SS.E.Eff _ -> failwith "should have been handled by the memory model"  
       
 
