src/coq/Effects.v
@@ -39,7 +39,7 @@ Inductive effects (d:Type) : Type :=
 | Alloca (t:typ)  (k:value -> d)        (* Stack allocation *)
 | Load   (a:addr) (k:value -> d)
 | Store  (a:addr) (v:value) (k:d)
-| Call   (v:value) (k:value -> d)
+| Call   (v:value) (args:list value) (k:value -> d)
 .    
 
 Definition effects_map {A B} (f:A -> B) (m:effects A) : effects B :=
@@ -47,7 +47,7 @@ Definition effects_map {A B} (f:A -> B) (m:effects A) : effects B :=
   | Alloca t g => Alloca t (fun a => f (g a))
   | Load a g  => Load a (fun dv => f (g dv))
   | Store a dv d => Store a dv (f d)
-  | Call a d => Call a (fun dv => f (d dv))
+  | Call v args d => Call v args (fun dv => f (d dv))
   end.
 
 Instance effects_functor : Functor effects := fun A => fun B => @effects_map A B.
@@ -68,18 +68,18 @@ CoInductive Obs X :=
 | Eff : effects (Obs X) -> Obs X    (* Externally visible step of computation *)
 .
 
-CoFixpoint d_map {A B} (f:A -> B) (d:Obs A) : Obs B :=
+CoFixpoint obs_map {A B} (f:A -> B) (d:Obs A) : Obs B :=
   match d with
     | Ret a => Ret (f a)
     | Fin d => Fin d
     | Err s => Err s
-    | Tau d' => Tau (d_map f d')
-    | Eff m => Eff (effects_map (d_map f) m)
+    | Tau d' => Tau (obs_map f d')
+    | Eff m => Eff (effects_map (obs_map f) m)
   end.
 
 Section UNFOLDING.
 
-Definition id_match_d {A} (d:Obs A) : Obs A :=
+Definition id_match_obs {A} (d:Obs A) : Obs A :=
   match d with
     | Ret a => Ret a
     | Fin d => Fin d
@@ -88,85 +88,85 @@ Definition id_match_d {A} (d:Obs A) : Obs A :=
     | Eff m => Eff m
   end.
 
-Lemma id_d_eq : forall A (d:Obs A),
-  d = id_match_d d.
+Lemma id_obs_eq : forall A (d:Obs A),
+  d = id_match_obs d.
 Proof.
   destruct d; auto.
 Qed.
 
 End UNFOLDING.
 
-Arguments id_d_eq {_} _ .
+Arguments id_obs_eq {_} _ .
 
 
-(* Error predicate, which says whether an observation trace leads to an error allong *)
-Inductive d_error_free_mem_step {A} (R: Obs A -> Prop) : effects (Obs A) -> Prop :=
-| d_error_free_mem_Alloca : forall t f, (forall (a:addr), R (f (inj_addr a))) -> d_error_free_mem_step R (Alloca t f)
-| d_error_free_mem_Load   : forall a f, (forall (dv:value), R (f dv)) -> d_error_free_mem_step R (Load a f)
-| d_error_free_mem_Store  : forall a n d, R d -> d_error_free_mem_step R (Store a n d)
-| d_error_free_mem_Call   : forall v f, (forall (dv:value), R (f dv)) -> d_error_free_mem_step R (Call v f)
+(* Error predicate, which says whether an observation trace leads to an error *)
+Inductive obs_error_free_mem_step {A} (R: Obs A -> Prop) : effects (Obs A) -> Prop :=
+| obs_error_free_mem_Alloca : forall t f, (forall (a:addr), R (f (inj_addr a))) -> obs_error_free_mem_step R (Alloca t f)
+| obs_error_free_mem_Load   : forall a f, (forall (dv:value), R (f dv)) -> obs_error_free_mem_step R (Load a f)
+| obs_error_free_mem_Store  : forall a n d, R d -> obs_error_free_mem_step R (Store a n d)
+| obs_error_free_mem_Call   : forall v vs f, (forall (dv:value), R (f dv)) -> obs_error_free_mem_step R (Call v vs f)
 .                                                                                
 
 (* No cases for Ret or Err --
    Ret means an "unfinished" computation (and shouldn't arise in the semantics of a CFG program)
    Err definitely has an error, which this predicate rules out
 *)
-Inductive d_error_free_step {A} (R:Obs A -> Prop) : Obs A -> Prop :=
-| d_error_free_step_fin : forall v, d_error_free_step R (Fin v)
-| d_error_free_step_tau : forall d, R d -> d_error_free_step R (Tau d)
-| d_error_free_step_eff : forall m, d_error_free_mem_step R m -> d_error_free_step R (Eff m)
+Inductive obs_error_free_step {A} (R:Obs A -> Prop) : Obs A -> Prop :=
+| obs_error_free_step_fin : forall v, obs_error_free_step R (Fin v)
+| obs_error_free_step_tau : forall d, R d -> obs_error_free_step R (Tau d)
+| obs_error_free_step_eff : forall m, obs_error_free_mem_step R m -> obs_error_free_step R (Eff m)
 .                                                                             
-Hint Constructors d_error_free_mem_step d_error_free_step.
+Hint Constructors obs_error_free_mem_step obs_error_free_step.
 
-Definition d_error_free {A} := paco1 (@d_error_free_step A) bot1.
-Hint Unfold d_error_free.
+Definition obs_error_free {A} := paco1 (@obs_error_free_step A) bot1.
+Hint Unfold obs_error_free.
 
-Lemma d_error_free_gen_mon {A} : monotone1 (@d_error_free_step A).
+Lemma obs_error_free_gen_mon {A} : monotone1 (@obs_error_free_step A).
 Proof.
   unfold monotone1. intros.
   induction IN; eauto.
-  eapply d_error_free_step_eff.
+  eapply obs_error_free_step_eff.
   induction H; constructor; auto.
 Qed.
-Hint Resolve d_error_free_gen_mon : paco.
+Hint Resolve obs_error_free_gen_mon : paco.
 
 (*
   This relation doesn't allow any variation in the relations for the memory model.  A more parametric version would:
     - have an address relation  A : addr -> addr -> Prop  
     - have a value relation  V : value -> value -> Prop
 *)
-Inductive d_equiv_mem_step {A} (R:Obs A -> Obs A -> Prop) : effects (Obs A) -> effects (Obs A) -> Prop :=
-| d_equiv_mem_Alloca : forall t f g, (forall (a:addr), R (f (inj_addr a)) (g (inj_addr a))) -> d_equiv_mem_step R (Alloca t f) (Alloca t g)
-| d_equiv_mem_Load  : forall a f g, (forall (dv:value), R (f dv) (g dv)) -> d_equiv_mem_step R (Load a f) (Load a g)
-| d_equiv_mem_Store : forall a n d1 d2, (R d1 d2) -> d_equiv_mem_step R (Store a n d1) (Store a n d2)
-| d_equiv_mem_Call  : forall v f g, (forall (dv:value), R (f dv) (g dv)) -> d_equiv_mem_step R (Call v f) (Call v g)
+Inductive obs_equiv_mem_step {A} (R:Obs A -> Obs A -> Prop) : effects (Obs A) -> effects (Obs A) -> Prop :=
+| obs_equiv_mem_Alloca : forall t f g, (forall (a:addr), R (f (inj_addr a)) (g (inj_addr a))) -> obs_equiv_mem_step R (Alloca t f) (Alloca t g)
+| obs_equiv_mem_Load  : forall a f g, (forall (dv:value), R (f dv) (g dv)) -> obs_equiv_mem_step R (Load a f) (Load a g)
+| obs_equiv_mem_Store : forall a n d1 d2, (R d1 d2) -> obs_equiv_mem_step R (Store a n d1) (Store a n d2)
+| obs_equiv_mem_Call  : forall v vs f g, (forall (dv:value), R (f dv) (g dv)) -> obs_equiv_mem_step R (Call v vs f) (Call v vs g)
 .    
 
-Inductive d_equiv_step {A} (R:Obs A -> Obs A -> Prop) : Obs A -> Obs A -> Prop :=
-| d_equiv_step_ret : forall a, d_equiv_step R (Ret a) (Ret a)
-| d_equiv_step_fin : forall v, d_equiv_step R (Fin v) (Fin v)
-| d_equiv_step_err : forall s1 s2, d_equiv_step R (Err s1) (Err s2)
-| d_equiv_step_tau : forall d1 d2, R d1 d2 -> d_equiv_step R (Tau d1) (Tau d2)
-| d_equiv_step_lft : forall d1 d2, d_equiv_step R d1 d2 -> d_equiv_step R (Tau d1) d2
-| d_equiv_step_rgt : forall d1 d2, d_equiv_step R d1 d2 -> d_equiv_step R d1 (Tau d2)
-| d_equiv_step_eff : forall m1 m2, d_equiv_mem_step R m1 m2 -> d_equiv_step R (Eff m1) (Eff m2)
+Inductive obs_equiv_step {A} (R:Obs A -> Obs A -> Prop) : Obs A -> Obs A -> Prop :=
+| obs_equiv_step_ret : forall a, obs_equiv_step R (Ret a) (Ret a)
+| obs_equiv_step_fin : forall v, obs_equiv_step R (Fin v) (Fin v)
+| obs_equiv_step_err : forall s1 s2, obs_equiv_step R (Err s1) (Err s2)
+| obs_equiv_step_tau : forall d1 d2 (equiv:R d1 d2), obs_equiv_step R (Tau d1) (Tau d2)
+| obs_equiv_step_lft : forall d1 d2, obs_equiv_step R d1 d2 -> obs_equiv_step R (Tau d1) d2
+| obs_equiv_step_rgt : forall d1 d2, obs_equiv_step R d1 d2 -> obs_equiv_step R d1 (Tau d2)
+| obs_equiv_step_eff : forall m1 m2, obs_equiv_mem_step R m1 m2 -> obs_equiv_step R (Eff m1) (Eff m2)
 .    
 
-Hint Constructors d_equiv_mem_step d_equiv_step.  (* d_equiv *)
+Hint Constructors obs_equiv_mem_step obs_equiv_step.  (* obs_equiv *)
 
-Lemma d_equiv_gen_mon A : monotone2 (@d_equiv_step A).
+Lemma obs_equiv_gen_mon A : monotone2 (@obs_equiv_step A).
 Proof.
   unfold monotone2. intros. induction IN; eauto.
-  eapply d_equiv_step_eff. induction H.
+  eapply obs_equiv_step_eff. induction H.
   - constructor. eauto.
   - constructor. eauto.
   - constructor. eauto.
   - constructor. eauto.
 Qed.
-Hint Resolve d_equiv_gen_mon : paco.
+Hint Resolve obs_equiv_gen_mon : paco.
 
-Definition d_equiv {A} (p q: Obs A) := paco2 (@d_equiv_step A) bot2 p q.
-Hint Unfold d_equiv.
+Definition obs_equiv {A} (p q: Obs A) := paco2 (@obs_equiv_step A) bot2 p q.
+Hint Unfold obs_equiv.
 
 Fixpoint taus {A} (n:nat) (d:Obs A) : Obs A :=
   match n with
@@ -174,30 +174,30 @@ Fixpoint taus {A} (n:nat) (d:Obs A) : Obs A :=
   | S n => Tau (taus n d)
   end.
 
-Instance D_functor : @Functor Obs := fun A => fun B => @d_map A B.
+Instance Obs_functor : @Functor Obs := fun A => fun B => @obs_map A B.
 
 
 (* A functor only up to stuttering equivalence. *)
 (*
-Program Instance D_functor_eq_laws : (@FunctorLaws D) D_functor (@d_equiv).
+Program Instance OBS_functor_eq_laws : (@FunctorLaws D) OBS_functor (@obs_equiv).
 *)
-Lemma d_equiv_refl : forall {A} (d : Obs A), d_equiv d d.
+Lemma obs_equiv_refl : forall {A}, reflexive (Obs A) obs_equiv.
 Proof.
-  intro. pcofix CIH.
-  intros. pfold. destruct d; eauto.
-  destruct e; eauto. 
+  intro A. pcofix CIH. intro d.
+  pfold. destruct d; eauto.
+  - destruct e; eauto. 
 Qed.
 
-Lemma d_equiv_symm : forall {A} (d1 d2 : Obs A), d_equiv d1 d2 -> d_equiv d2 d1.
+Lemma obs_equiv_symm : forall {A}, symmetric (Obs A) obs_equiv.
 Proof.
   intro. pcofix CIH.
   intros d1 d2 H.
-  punfold H. remember (upaco2 d_equiv_step bot2).
+  punfold H. remember (upaco2 obs_equiv_step bot2).
   induction H; eauto; subst.
   - pfold. constructor. right. eapply CIH.
-    destruct H; eauto. inversion H. 
-  - pfold. constructor. punfold IHd_equiv_step.
-  - pfold. constructor. punfold IHd_equiv_step.
+    destruct equiv; eauto. inversion H. 
+  - pfold. constructor. punfold IHobs_equiv_step.
+  - pfold. constructor. punfold IHobs_equiv_step.
   - pfold. constructor. inversion H; subst.
     + constructor. intro. specialize (H0 a). destruct H0.
       right. eapply CIH. eapply H0. inversion H0.
@@ -207,6 +207,83 @@ Proof.
     + constructor. intro. specialize (H0 dv). destruct H0.
       right. eapply CIH. eapply H0. inversion H0.
 Qed.
+
+
+Lemma obs_equiv_lft_inversion : forall {A} (d1 d2:Obs A), obs_equiv (Tau d1) d2 -> obs_equiv d1 d2.
+Proof.
+  intros A d1 d2 H.  punfold H. remember (Tau d1) as d. induction H; try (inversion Heqd; subst; clear Heqd).
+  - pfold. constructor. pclearbot. 
+    destruct equiv. eapply obs_equiv_gen_mon.
+    eapply SIM. eapply LE.
+  - pfold. eapply H.
+  - pfold. constructor.
+    apply IHobs_equiv_step in Heqd.
+    punfold Heqd.
+Qed. 
+
+Lemma stutter_simpl : forall {A} (d1 d2: Obs A) n, obs_equiv (taus n d1) d2 -> obs_equiv d1 d2.
+Proof.
+  intros. induction n. punfold H.
+  eapply IHn. simpl in H. eapply obs_equiv_lft_inversion. eapply H.
+Qed.
+
+Lemma stutter : forall {A} (d1 d2: Obs A) n m, obs_equiv (taus n d1) (taus m d2) -> obs_equiv d1 d2.
+Proof.
+  intros.
+  eapply stutter_simpl.
+  eapply obs_equiv_symm.
+  eapply stutter_simpl.
+  eapply obs_equiv_symm.
+  eauto.
+Qed.
+
+
+Lemma obs_equiv_step_transitive:  forall A R, transitive (Obs A) R -> transitive (Obs A) (obs_equiv_step R).
+Proof.
+  intros A.
+  unfold relation. unfold transitive.
+  intros R Ht.
+  intros x y z H. generalize dependent z.
+  induction H; intros z H1. 
+  - remember (Ret a) as w. induction H1; inversion Heqw; eauto.
+    subst. apply obs_equiv_step_rgt. exact H1.
+  - remember (Fin v) as w. induction H1; inversion Heqw; eauto.
+    subst. apply obs_equiv_step_rgt. exact H1.
+  - remember (Err s2) as w. induction H1; inversion Heqw; eauto.
+  - apply obs_equiv_step_lft. generalize dependent d1. remember (Tau d2) as w.
+    induction H1; inversion Heqw; subst; intros d1 HR.
+    apply obs_equiv_step_rgt. 
+Abort.    
+  
+
+
+Lemma obs_equiv_trans : forall {A} (d1 d2 d3: Obs A), obs_equiv d1 d2 -> obs_equiv d2 d3 -> obs_equiv d1 d3.
+Proof.
+  intro A. pcofix CIH.
+  intros d1 d2 d3 H1 H2.
+  pfold.
+  punfold H1. remember (upaco2 obs_equiv_step bot2) as R.
+  generalize dependent d3.
+  induction H1; intros d3 H2.
+  - punfold H2. rewrite <- HeqR in H2. remember (Ret a) as d2.
+    induction H2; try inversion Heqd2; eauto.
+    apply obs_equiv_step_rgt. subst. apply IHobs_equiv_step in H.  exact H.
+  - punfold H2. rewrite <- HeqR in H2. remember (Fin v) as d2.
+    induction H2; try inversion Heqd2; eauto.
+    apply obs_equiv_step_rgt. subst. apply IHobs_equiv_step in H. exact H.
+  - punfold H2. rewrite <- HeqR in H2. remember (Err s2) as d2.
+    induction H2; try inversion Heqd2; eauto.
+  - punfold H2.
+    rewrite <- HeqR in H2. remember (Tau d2) as d.
+    induction H2; try inversion Heqd; subst; eauto.
+    + pclearbot. destruct equiv. destruct equiv0.
+    apply obs_equiv_step_tau. right. eapply CIH. pfold.
+    eapply obs_equiv_gen_mon. apply SIM. eapply LE.
+    pfold. eapply obs_equiv_gen_mon. eapply SIM0. eapply LE0.
+    + pclearbot. destruct equiv. 
+      apply obs_equiv_step_lft.  eapply obs_equiv_gen_mon.
+Abort.
+      
 
 (* Note: for guardedness, bind Ret introduces extra Tau *)
 Definition bind {A B} (m:Obs A) (f:A -> Obs B) : Obs B :=
@@ -219,8 +296,8 @@ Definition bind {A B} (m:Obs A) (f:A -> Obs B) : Obs B :=
        | Eff m => Eff (effects_map bindf m)
      end) m.
 
-Lemma bind_unfold : forall {A B} (m:Obs A) (f:A -> Obs B),
-    d_equiv (bind m f)
+Lemma binobs_unfold : forall {A B} (m:Obs A) (f:A -> Obs B),
+    obs_equiv (bind m f)
     (match m with
     | Ret a => Tau (f a)
     | Fin d => Fin d
@@ -231,6 +308,8 @@ Lemma bind_unfold : forall {A B} (m:Obs A) (f:A -> Obs B),
 Proof.
   intros A B.
   pcofix CIH. intros m f.
+  unfold bind.
+  pfold. destruct m.
 Abort.
   
 Program Instance Obs_monad : (@Monad Obs) (@Obs_functor) := _.
@@ -255,10 +334,10 @@ Section OBS_EQUIV_COIND.
   Variables (p:Obs A) (q:Obs A).
   Hypothesis Hrpq : R p q.
   Hypothesis H : forall d1 d2,
-    R d1 d2 -> d_equiv_step R d1 d2.
+    R d1 d2 -> obs_equiv_step R d1 d2.
   
-  Theorem d_equiv_coind :
-    d_equiv p q.
+  Theorem obs_equiv_coind :
+    obs_equiv p q.
   Proof.
     revert p q Hrpq.
     pcofix CIH.
@@ -279,35 +358,8 @@ Section OBS_EQUIV_COIND.
   Qed.
 
 End OBS_EQUIV_COIND.
-Arguments d_equiv_coind [_] _ [_ _] _ _.
+Arguments obs_equiv_coind [_] _ [_ _] _ _.
 
 
-Lemma stutter_helper : forall {A} (d1 d2: Obs A), d_equiv (Tau d1) d2 -> d_equiv d1 d2.
-Proof.
-  intros A d1 d2 H.  punfold H. remember (Tau d1). induction H; try (solve [inversion Heqo]).
-  - inversion Heqo; subst. pfold. constructor. unfold upaco2 in H.
-    destruct H; inversion H. eapply d_equiv_gen_mon.
-    eapply SIM. eapply LE.
-  - inversion Heqo; subst. pfold. eapply H.
-  - inversion Heqo; subst. pfold. constructor.
-    eapply IHd_equiv_step in H0. punfold H0.
-Qed. 
-
-Lemma stutter_simpl : forall {A} (d1 d2: Obs A) n, d_equiv (taus n d1) d2 -> d_equiv d1 d2.
-Proof.
-  intros. induction n. punfold H.
-  eapply IHn. simpl in H. eapply stutter_helper. eapply H.
-Qed.
-
-
-Lemma stutter : forall {A} (d1 d2: Obs A) n m, d_equiv (taus n d1) (taus m d2) -> d_equiv d1 d2.
-Proof.
-  intros.
-  eapply stutter_simpl.
-  eapply d_equiv_symm.
-  eapply stutter_simpl.
-  eapply d_equiv_symm.
-  eauto.
-Qed.
 
 End Effects.
