src/coq/CompilerProp.v
@@ -10,8 +10,9 @@
 
 Require Import Vellvm.Maps Vellvm.Imp.
 
-(* Require Import QuickChick.QuickChick. *)
-(* Import QcDefaultNotation. Open Scope qc_scope. *)
+Require Import QuickChick.QuickChick. 
+Import QcDefaultNotation. Open Scope qc_scope. 
+
 Require Import List ZArith.
 Import ListNotations.
 Require Import String.
@@ -57,12 +58,11 @@ Fixpoint imp_memory_eqb (m1 : list dvalue) (m2 : list dvalue) : bool :=
  *)
 Require Import List.
 
-(*
+
 Definition state_to_string (st : state) (fv : list id) : string :=
   fold_left (fun acc x => (match x with
-                        | Id ident => (ident ++ ": " ++ string_of (st x) ++ ", ")%string
+                        | Id ident => (ident ++ ": " ++ show (st x) ++ ", ")%string
                         end)) fv "".
-*)
 
 
 Definition imp_compiler_correct_aux (p:Imp.com) :=
@@ -98,7 +98,6 @@ Definition another_imp_compiler_correct (p:Imp.com) : string * bool :=
   match compile p with
   | inl e => ("Compilation failed", false)
   | inr ll_prog =>
-    (*
     let m := modul_of_toplevel_entities ll_prog in
     match mcfg_of_modul m with
     | None => ("Compilation failed", false)
@@ -109,8 +108,7 @@ Definition another_imp_compiler_correct (p:Imp.com) : string * bool :=
         let semantics := sem mcfg initial_state in
         ("Success", true)
       end        
-    end*)
-    ("Success", true)
+    end
   end.
 
 Example prog1 := W ::= AId W.
@@ -118,7 +116,6 @@ Example prog2 := X ::= APlus (AId W) (AId W).
 
 
 Eval vm_compute in (compile prog2).
-
 Eval vm_compute in (another_imp_compiler_correct prog1).
 
 
